src/theta_tree.v
@@ -1,0 +1,76 @@
+Require Import definitions.
+Require Import Nat.
+
+Inductive SomeKindaTree : Type :=
+| t_inner (eest: nat) (energy: nat) (nvlpc: nat)
+          (lhs: SomeKindaTree) (rhs: SomeKindaTree) : SomeKindaTree
+| t_leaf (energy: nat) (nvlpc: nat) : SomeKindaTree.
+
+Definition ThetaTree := SomeKindaTree.
+Axiom tree_insert : forall (t: ThetaTree) (n: Activity), ThetaTree.
+
+Axiom split_at : forall (node: SomeKindaTree) (est_split: nat),
+  (SomeKindaTree * SomeKindaTree).
+
+Definition tree_energy (node: SomeKindaTree) := match node with
+| t_inner _ energy _ _ _ => energy
+| t_leaf energy _ => energy
+end.
+
+Definition nvlpc (node: SomeKindaTree) := match node with
+| t_inner _ _ nvlpc _ _ => nvlpc
+| t_leaf _ nvlpc => nvlpc
+end.
+
+Fixpoint eval_maxest_i
+  (task_lct: nat)
+  (C_c: nat)
+  (E: nat)
+  (node: SomeKindaTree)
+:
+  nat
+:=
+  match node with
+  | t_leaf eest _ => eest
+  | t_inner eest _ _ lhs rhs =>
+    if (C_c) * task_lct <? nvlpc rhs + E then
+      eval_maxest_i task_lct C_c E rhs
+    else
+      eval_maxest_i task_lct C_c (E+tree_energy rhs) lhs
+  end.
+
+Definition eval_maxest (C: nat) (c: nat) (task_lct: nat) (root: SomeKindaTree) :=
+  eval_maxest_i task_lct (C-c) 0 root.
+
+(*
+
+Definition isMaxOfFunctionOverType
+    {A: Type} (p : A -> Prop) (f: A -> nat) (max: nat) : Prop :=
+  (forall (a: A), p a -> f a <= max) /\ (exists (a: A), p a /\ f a = max).
+
+Inductive SortedTree (A: Type) (rel: A -> A -> Prop) : list A -> A -> Type :=
+| o_leaf (a: A) : SortedTree A rel (cons a nil) a
+| o_node {ll lr} {l r} (lhs: SortedTree A rel ll l) (rhs: SortedTree A rel lr r) :
+  rel l r -> SortedTree A rel (ll++lr) l.
+
+Definition est_le {A} `{Work A} (a b: A) := (est a) <= (est b).
+
+Definition ThetaTree := SortedTree Activity est_le.
+
+Fixpoint theta_tree_energy {l a} (t: ThetaTree l a) : nat := match t with
+| o_leaf _ _ activity => est activity
+| o_node _ _ lhs rhs related => (theta_tree_energy lhs) + (theta_tree_energy rhs)
+end.
+
+Fixpoint theta_tree_envelope {l a} (C: nat) (t: ThetaTree l a) : nat := match t with
+| o_leaf _ _ activity => (est activity) * C + (energy activity)
+| o_node _ _ lhs rhs related =>
+    max
+    (theta_tree_envelope C lhs + theta_tree_energy rhs)
+    (theta_tree_envelope C rhs)
+end.
+
+Definition envelope_op (C: nat) (energy_a envelope_a energy_b envelope_b) :=
+  (energy_a + energy_b, max (envelope_a + energy_a) envelope_b).
+
+*)
